examples/tutorial/6-smt/tutorialExtra2_smtScript.sml
@@ -1,0 +1,41 @@
+open HolKernel Parse boolLib bossLib;
+
+open bir_expSyntax;
+open bir_exp_tautologiesTheory;
+
+(* From shared: *)
+open bir_exp_to_wordsLib bslSyntax;
+open pretty_exnLib;
+
+(* From examples: *)
+open tutorialExtra2_wpTheory;
+open tutorial_smtSupportLib;
+
+
+val _ = new_theory "tutorialExtra2_smt";
+
+
+
+val h_var_v1 = mk_var ("v1", Type `:word32`);
+
+val get_contract_vars = (lhs o concl o (SPEC h_var_v1));
+
+
+val contract_1_pre = get_contract_vars bir_ieo_sec_iseven_1_pre_def;
+val contract_1_wp  = get_contract_vars bir_ieo_sec_iseven_1_wp_def;
+val contract_1_imp = bimp (contract_1_pre, contract_1_wp);
+
+val contract_1_imp_taut_thm = save_thm ("contract_1_imp_taut_thm",
+  prove_exp_is_taut contract_1_imp);
+
+
+val contract_2_pre = get_contract_vars bir_ieo_sec_isodd_1_pre_def;
+val contract_2_wp  = get_contract_vars bir_ieo_sec_isodd_1_wp_def;
+val contract_2_imp = bimp (contract_2_pre, contract_2_wp);
+
+val contract_2_imp_taut_thm = save_thm ("contract_2_imp_taut_thm",
+  prove_exp_is_taut contract_2_imp);
+
+
+val _ = export_theory();
+
