examples/tutorial/7-composition/tutorialExtra2_compositionScript.sml
@@ -1,0 +1,73 @@
+open HolKernel Parse boolLib bossLib;
+open bslSyntax;
+open birExamplesBinaryTheory;
+open bir_wm_instTheory;
+open bin_hoare_logicTheory;
+open bir_valuesTheory;
+open bir_bool_expTheory;
+open bir_auxiliaryTheory;
+open bir_exp_equivTheory;
+open bir_programTheory;
+
+open tutorial_compositionLib;
+open tutorial_wpSupportLib;
+
+open tutorialExtra2_wpTheory;
+open tutorialExtra2_smtTheory;
+
+open bir_auxiliaryLib;
+
+open HolBACoreSimps;
+open HolBASimps;
+open bin_hoare_logicSimps;
+
+val _ = new_theory "tutorialExtra2_composition";
+
+(************************************)
+(* TODO: Where to place the below? *)
+fun el_in_set elem set =
+  EQT_ELIM (SIMP_CONV (std_ss++pred_setLib.PRED_SET_ss) [] (pred_setSyntax.mk_in (elem, set)));
+
+val mk_set = pred_setSyntax.mk_set;
+
+val simp_delete_set_rule =
+  SIMP_RULE (std_ss++pred_setLib.PRED_SET_ss++HolBACoreSimps.holBACore_ss++wordsLib.WORD_ss)
+    [pred_setTheory.DELETE_DEF]
+
+val simp_insert_set_rule =
+  SIMP_RULE (std_ss++pred_setLib.PRED_SET_ss++HolBACoreSimps.holBACore_ss++wordsLib.WORD_ss)
+    [(* ??? *)]
+
+val simp_in_sing_set_rule =
+  SIMP_RULE std_ss [pred_setTheory.IN_SING]
+
+fun simp_inter_set_rule ht =
+  ONCE_REWRITE_RULE [EVAL (get_bir_map_triple_blist ht)] ht
+
+val simp_in_set_tac =
+  SIMP_TAC (std_ss++HolBACoreSimps.holBACore_ss++wordsLib.WORD_ss++pred_setLib.PRED_SET_ss) []
+
+(* DEBUG *)
+val (get_labels_from_set_repr, el_in_set_repr,
+     mk_set_repr, simp_delete_set_repr_rule,
+     simp_insert_set_repr_rule, simp_in_sing_set_repr_rule, simp_inter_set_repr_rule, simp_in_set_repr_tac, inter_set_repr_ss, union_set_repr_ss) = (ending_set_to_sml_list, el_in_set, mk_set, simp_delete_set_rule,
+     simp_insert_set_rule, simp_in_sing_set_rule, simp_inter_set_rule, simp_in_set_tac, bir_inter_var_set_ss, bir_union_var_set_ss);
+(************************************)
+
+(* =============================================================== *)
+
+val bir_ieo_sec_iseven_1_comp_ht =
+  use_pre_str_rule
+    (HO_MATCH_MP bir_label_ht_impl_weak_ht bir_ieo_sec_iseven_1_ht)
+    contract_1_imp_taut_thm;
+
+val bir_ieo_sec_isodd_1_comp_ht =
+  use_pre_str_rule
+    (HO_MATCH_MP bir_label_ht_impl_weak_ht bir_ieo_sec_isodd_1_ht)
+    contract_2_imp_taut_thm;
+
+
+(* =============================================================== *)
+
+
+val _ = export_theory();
